Faster proofs for TwoLevelSimp

Valaig/Aig/TwoLevelSimp.lean
@@ -1,6 +1,8 @@
 module
 
 public import Valaig.Refs
+import Std.Tactic.Do
+import Std.Do
 
 public section
 namespace Valaig.Aig
@@ -12,8 +14,8 @@ Minimization without Blowup" by Brummayer and Biere.
 -/
 
 variable (assign : Lit -> Bool)
-variable {assignInv : ∀ lit, assign lit = (lit.inverted ^^ assign lit.strip)}
-variable {assignFalse : assign .false = .false}
+variable {assignInv : ∀ (lit : Lit), assign lit.invert = !assign lit}
+variable {assignConst : ∀ inv, assign (.mk .constant inv) = inv}
 
 inductive SimplifiedAnd where
 | lit : Lit -> SimplifiedAnd
@@ -28,6 +30,10 @@ def denote (assign : Lit -> Bool) : SimplifiedAnd -> Bool
 
 end SimplifiedAnd
 
+-- Used for mvcgen proofs
+open Std.Do
+set_option mvcgen.warning false
+
 @[inline]
 def constFoldLeft (lhs rhs : Lit) : Option Lit := do
   if ¬lhs.isConstant then
@@ -35,20 +41,29 @@ def constFoldLeft (lhs rhs : Lit) : Option Lit := do
 
   -- Boundedness: (⊥ ∧ r) = ⊥
   if lhs = .false then
-    return false
+    return .false
   -- Neutrality: (⊤ ∧ r) = r
   else
     return rhs
 
-include assignInv assignFalse in
+include assignConst in
 theorem denote_constFoldLeft {lhs rhs out : Lit} (heq : constFoldLeft lhs rhs = some out) :
     assign out = (assign lhs && assign rhs) := by
-  grind [constFoldLeft]
+  revert heq
+  generalize h : constFoldLeft lhs rhs = res
+  apply Option.of_wp_eq h
+  unfold constFoldLeft
+  mvcgen with (cbv; grind)
 
-@[grind →]
-theorem values_constFoldLeft {lhs rhs out : Lit} (heq : constFoldLeft lhs rhs = some out) :
-    out.isConstant ∨ out.var = lhs.var ∨ out.var = rhs.var := by
-  grind [constFoldLeft]
+theorem var_constFoldLeft {lhs rhs out : Lit} (motive : Var -> Prop)
+    (heq : constFoldLeft lhs rhs = some out)
+    (hconst : motive .constant) (hrhs : motive rhs.var) :
+    motive out.var := by
+  revert heq
+  generalize h : constFoldLeft lhs rhs = res
+  apply Option.of_wp_eq h
+  unfold constFoldLeft
+  mvcgen with (cbv; grind)
 
 @[inline]
 def constFold (lhs rhs : Lit) : Option Lit := do
@@ -60,16 +75,30 @@ def constFold (lhs rhs : Lit) : Option Lit := do
 
   none
 
-include assignInv assignFalse in
+include assignConst in
 theorem denote_constFold {lhs rhs out : Lit} (heq : constFold lhs rhs = some out) :
     assign out = (assign lhs && assign rhs) := by
-  have := @denote_constFoldLeft assign
-  grind [constFold]
+  revert heq
+  generalize h : constFold lhs rhs = res
+  apply Option.of_wp_eq h
+  unfold constFold
+  mvcgen
+  next heq => grind [denote_constFoldLeft assign (heq := heq)]
+  next heq => grind [denote_constFoldLeft assign (heq := heq)]
+  next => cbv; grind
 
-@[grind →]
-theorem values_constFold {lhs rhs out : Lit} (heq : constFold lhs rhs = some out) :
-    out.isConstant ∨ out.var = lhs.var ∨ out.var = rhs.var := by
-  grind [constFold]
+theorem var_constFold {lhs rhs out : Lit} (motive : Var -> Prop)
+    (heq : constFold lhs rhs = some out)
+    (hconst : motive .constant) (hlhs : motive lhs.var) (hrhs : motive rhs.var) :
+    motive out.var := by
+  revert heq
+  generalize h : constFold lhs rhs = res
+  apply Option.of_wp_eq h
+  unfold constFold
+  mvcgen
+  next heq => grind [var_constFoldLeft motive heq]
+  next heq => grind [var_constFoldLeft motive heq]
+  next => cbv; grind
 
 @[inline]
 def twoInput (lhs rhs : Lit) : Option Lit := do
@@ -82,20 +111,32 @@ def twoInput (lhs rhs : Lit) : Option Lit := do
 
   -- Contradiction: (l ∧ ¬l) = ⊥
   if lhs = rhs.invert then
-    return false
+    return .false
 
   none
 
-include assignInv assignFalse in
+include assignInv assignConst in
 theorem denote_twoInput {lhs rhs out : Lit} (heq : twoInput lhs rhs = some out) :
     assign out = (assign lhs && assign rhs) := by
-  have := @denote_constFold assign
-  grind [twoInput]
+  revert heq
+  generalize h : twoInput lhs rhs = res
+  apply Option.of_wp_eq h
+  unfold twoInput
+  mvcgen
+  next heq => grind [denote_constFold assign (heq := heq)]
+  next heq => grind
+  next heq => grind
+  next => cbv; grind
 
-@[grind →]
-theorem values_twoInput {lhs rhs out : Lit} (heq : twoInput lhs rhs = some out) :
-    out.isConstant ∨ out.var = lhs.var ∨ out.var = rhs.var := by
-  grind [twoInput]
+theorem var_twoInput {lhs rhs out : Lit} (motive : Var -> Prop)
+    (heq : twoInput lhs rhs = some out)
+    (hconst : motive .constant) (hlhs : motive lhs.var) (hrhs : motive rhs.var) :
+    motive out.var := by
+  revert heq
+  generalize h : twoInput lhs rhs = res
+  apply Option.of_wp_eq h
+  unfold twoInput
+  mvcgen with (cbv; grind [var_constFold motive])
 
 @[inline]
 def threeInputLeftNeg (rhs l0 l1 : Lit) : Option SimplifiedAnd := do
@@ -117,64 +158,64 @@ include assignInv in
 theorem denote_threeInputLeftNeg {rhs l0 l1 : Lit} {out : SimplifiedAnd}
     (heq : threeInputLeftNeg rhs l0 l1 = some out) :
     out.denote assign = (!(assign l0 && assign l1) && assign rhs) := by
-  simp [threeInputLeftNeg] at heq
-  grind 
+  revert heq
+  generalize h : threeInputLeftNeg rhs l0 l1 = res
+  apply Option.of_wp_eq h
+  unfold threeInputLeftNeg
+  mvcgen with (cbv; grind)
 
-@[grind →]
-theorem values_threeInputLeftNeg_lit {rhs l0 l1 out : Lit}
-    (heq : threeInputLeftNeg rhs l0 l1 = some (.lit out)) :
-    out.isConstant ∨ out.var = rhs.var ∨ out.var = l0.var ∨ out.var = l1.var := by
-  grind [threeInputLeftNeg]
+theorem var_threeInputLeftNeg_lit {rhs l0 l1 out : Lit} (motive : Var -> Prop)
+    (heq : threeInputLeftNeg rhs l0 l1 = some (.lit out))
+    (hrhs : motive rhs.var) :
+    motive out.var := by
+  revert heq
+  generalize h : threeInputLeftNeg rhs l0 l1 = res
+  apply Option.of_wp_eq h
+  unfold threeInputLeftNeg
+  mvcgen with (cbv; grind)
 
-@[grind →]
-theorem values_threeInputLeftNeg_and_lhs {rhs l0 l1 o0 o1 : Lit}
-    (heq : threeInputLeftNeg rhs l0 l1 = some (.and o0 o1)) :
-    o0.isConstant ∨ o0.var = rhs.var ∨ o0.var = l0.var ∨ o0.var = l1.var := by
-  grind [threeInputLeftNeg]
-
-@[grind →]
-theorem values_threeInputLeftNeg_and_rhs {rhs l0 l1 o0 o1 : Lit}
-    (heq : threeInputLeftNeg rhs l0 l1 = some (.and o0 o1)) :
-    o1.isConstant ∨ o1.var = rhs.var ∨ o1.var = l0.var ∨ o1.var = l1.var := by
-  grind [threeInputLeftNeg]
+theorem var_threeInputLeftNeg_and {rhs l0 l1 o0 o1 : Lit} (motive : Var -> Prop)
+    (heq : threeInputLeftNeg rhs l0 l1 = some (.and o0 o1))
+    (hl0 : motive l0.var) (hl1 : motive l1.var) :
+    motive o0.var ∧ motive o1.var := by
+  revert heq
+  generalize h : threeInputLeftNeg rhs l0 l1 = res
+  apply Option.of_wp_eq h
+  unfold threeInputLeftNeg
+  mvcgen with (cbv; grind)
 
 @[inline]
-def threeInputLeftPos (lhs rhs l0 l1 : Lit) : Option SimplifiedAnd := do
+def threeInputLeftPos (lhs rhs l0 l1 : Lit) : Option Lit := do
   -- Contradiction: (¬r ∧ l1) ∧ r = (l0 ∧ ¬r) ∧ r = ⊥
   if l0 = rhs.invert ∨ l1 = rhs.invert then
-    return .lit .false
+    return .false
 
   -- Idempotence: (l0 ∧ l1) ∧ l0 = (l0 ∧ l1) ∧ l1 = (l0 ∧ l1)
   if l0 = rhs ∨ l1 = rhs then
-    return .lit lhs
+    return lhs
 
   none
 
-include assignInv assignFalse in
-theorem denote_threeInputLeftPos {lhs rhs l0 l1 : Lit} {out : SimplifiedAnd}
+include assignInv assignConst in
+theorem denote_threeInputLeftPos {lhs rhs l0 l1 : Lit} {out : Lit}
     (heq : threeInputLeftPos lhs rhs l0 l1 = some out)
     (hl : assign lhs = (assign l0 && assign l1)) :
-    out.denote assign = (assign lhs && assign rhs) := by
-  simp [threeInputLeftPos] at heq
-  grind
+    assign out = (assign lhs && assign rhs) := by
+  revert heq
+  generalize h : threeInputLeftPos lhs rhs l0 l1 = res
+  apply Option.of_wp_eq h
+  unfold threeInputLeftPos
+  mvcgen with (cbv; grind)
 
-@[grind →]
-theorem values_threeInputLeftPos_lit {lhs rhs l0 l1 out : Lit}
-    (heq : threeInputLeftPos lhs rhs l0 l1 = some (.lit out)) :
-    out.isConstant ∨ out.var = lhs.var ∨ out.var = rhs.var ∨ out.var = l0.var ∨ out.var = l1.var := by
-  grind [threeInputLeftPos]
-
-@[grind →]
-theorem values_threeInputLeftPos_and_lhs {lhs rhs l0 l1 o0 o1 : Lit}
-    (heq : threeInputLeftPos lhs rhs l0 l1 = some (.and o0 o1)) :
-    o0.isConstant ∨ o0.var = lhs.var ∨ o0.var = rhs.var ∨ o0.var = l0.var ∨ o0.var = l1.var := by
-  grind [threeInputLeftPos]
-
-@[grind →]
-theorem values_threeInputLeftPos_and_rhs {lhs rhs l0 l1 o0 o1 : Lit}
-    (heq : threeInputLeftPos lhs rhs l0 l1 = some (.and o0 o1)) :
-    o1.isConstant ∨ o1.var = lhs.var ∨ o1.var = rhs.var ∨ o1.var = l0.var ∨ o1.var = l1.var := by
-  grind [threeInputLeftPos]
+theorem var_threeInputLeftPos {lhs rhs l0 l1 out : Lit} (motive : Var -> Prop)
+    (heq : threeInputLeftPos lhs rhs l0 l1 = some out)
+    (hconst : motive .constant) (hlhs : motive lhs.var) :
+    motive out.var := by
+  revert heq
+  generalize h : threeInputLeftPos lhs rhs l0 l1 = res
+  apply Option.of_wp_eq h
+  unfold threeInputLeftPos
+  mvcgen with (cbv; grind)
 
 @[inline]
 def threeInputLeft (lhs rhs l0 l1 : Lit) : Option SimplifiedAnd := do
@@ -183,39 +224,46 @@ def threeInputLeft (lhs rhs l0 l1 : Lit) : Option SimplifiedAnd := do
       return l
   else
     if let some l := threeInputLeftPos lhs rhs l0 l1 then
-      return l
+      return .lit l
 
   none
 
-include assignInv assignFalse in
+include assignInv assignConst in
 theorem denote_threeInputLeft {lhs rhs l0 l1 : Lit} {out : SimplifiedAnd}
     (heq : threeInputLeft lhs rhs l0 l1 = some out)
-    (hl : assign lhs.strip = (assign l0 && assign l1)) :
+    (hl : assign lhs = ((decide lhs.inverted) ^^ (assign l0 && assign l1))) :
     out.denote assign = (assign lhs && assign rhs) := by
-  simp [threeInputLeft] at heq
-  split at heq
-  · have := @denote_threeInputLeftNeg assign
-    grind
-  · have := @denote_threeInputLeftPos assign assignInv assignFalse lhs rhs l0 l1
-    grind
+  revert heq
+  generalize h : threeInputLeft lhs rhs l0 l1 = res
+  apply Option.of_wp_eq h
+  unfold threeInputLeft
+  mvcgen
+  next heq => grind [denote_threeInputLeftNeg assign (heq := heq)]
+  next => cbv; grind
+  next h _ heq =>
+    simp [h]at hl
+    grind [denote_threeInputLeftPos assign (heq := heq)]
+  next => cbv; grind
 
-@[grind →]
-theorem values_threeInputLeft_lit {lhs rhs l0 l1 out : Lit}
-    (heq : threeInputLeft lhs rhs l0 l1 = some (.lit out)) :
-    out.isConstant ∨ out.var = lhs.var ∨ out.var = rhs.var ∨ out.var = l0.var ∨ out.var = l1.var := by
-  grind [threeInputLeft]
+theorem var_threeInputLeft_lit {lhs rhs l0 l1 out : Lit} (motive : Var -> Prop)
+    (heq : threeInputLeft lhs rhs l0 l1 = some (.lit out))
+    (hconst : motive .constant) (hlhs : motive lhs.var) (hrhs : motive rhs.var) :
+    motive out.var := by
+  revert heq
+  generalize h : threeInputLeft lhs rhs l0 l1 = res
+  apply Option.of_wp_eq h
+  unfold threeInputLeft
+  mvcgen
+  next heq => grind [var_threeInputLeftNeg_lit motive]
+  next => cbv; grind
+  next h _ heq => grind [var_threeInputLeftPos motive]
+  next => cbv; grind
 
-@[grind →]
-theorem values_threeInputLeft_and_lhs {lhs rhs l0 l1 o0 o1 : Lit}
-    (heq : threeInputLeft lhs rhs l0 l1 = some (.and o0 o1)) :
-    o0.isConstant ∨ o0.var = lhs.var ∨ o0.var = rhs.var ∨ o0.var = l0.var ∨ o0.var = l1.var := by
-  grind [threeInputLeft]
-
-@[grind →]
-theorem values_threeInputLeft_and_rhs {lhs rhs l0 l1 o0 o1 : Lit}
-    (heq : threeInputLeft lhs rhs l0 l1 = some (.and o0 o1)) :
-    o1.isConstant ∨ o1.var = lhs.var ∨ o1.var = rhs.var ∨ o1.var = l0.var ∨ o1.var = l1.var := by
-  grind [threeInputLeft]
+theorem var_threeInputLeft_and {lhs rhs l0 l1 o0 o1 : Lit} (motive : Var -> Prop)
+    (heq : threeInputLeft lhs rhs l0 l1 = some (.and o0 o1))
+    (hl0 : motive l0.var) (hl1 : motive l1.var) :
+    motive o0.var ∧ motive o1.var := by
+  grind [threeInputLeft, var_threeInputLeftNeg_and motive]
 
 @[inline]
 def fourInputPosPos (lhs l0 l1 r0 r1 : Lit) : Option SimplifiedAnd := do
@@ -236,31 +284,36 @@ def fourInputPosPos (lhs l0 l1 r0 r1 : Lit) : Option SimplifiedAnd := do
 
   none
 
-include assignInv assignFalse in
+include assignInv assignConst in
 theorem denote_fourInputPosPos {lhs l0 l1 r0 r1 : Lit} {out : SimplifiedAnd}
     (heq : fourInputPosPos lhs l0 l1 r0 r1 = some out)
     (hl : assign lhs = (assign l0 && assign l1)) :
     out.denote assign = (assign lhs && (assign r0 && assign r1)) := by
-  simp [fourInputPosPos] at heq
-  grind
+  revert heq
+  generalize h : fourInputPosPos lhs l0 l1 r0 r1 = res
+  apply Option.of_wp_eq h
+  unfold fourInputPosPos
+  mvcgen with (cbv; grind)
 
-@[grind →]
-theorem values_fourInputPosPos_lit {lhs l0 l1 r0 r1 out : Lit}
-    (heq : fourInputPosPos lhs l0 l1 r0 r1 = some (.lit out)) :
-    out.isConstant ∨ out.var = lhs.var ∨ out.var = l0.var ∨ out.var = l1.var ∨ out.var = r0.var ∨ out.var = r1.var := by
-  grind [fourInputPosPos]
+theorem var_fourInputPosPos_lit {lhs l0 l1 r0 r1 out : Lit} (motive : Var -> Prop)
+    (heq : fourInputPosPos lhs l0 l1 r0 r1 = some (.lit out))
+    (hconst : motive .constant) :
+    motive out.var := by
+  revert heq
+  generalize h : fourInputPosPos lhs l0 l1 r0 r1 = res
+  apply Option.of_wp_eq h
+  unfold fourInputPosPos
+  mvcgen with (cbv; grind)
 
-@[grind →]
-theorem values_fourInputPosPos_and_lhs {lhs l0 l1 r0 r1 o0 o1 : Lit}
-    (heq : fourInputPosPos lhs l0 l1 r0 r1 = some (.and o0 o1)) :
-    o0.isConstant ∨ o0.var = lhs.var ∨ o0.var = l0.var ∨ o0.var = l1.var ∨ o0.var = r0.var ∨ o0.var = r1.var := by
-  grind [fourInputPosPos]
-
-@[grind →]
-theorem values_fourInputPosPos_and_rhs {lhs l0 l1 r0 r1 o0 o1 : Lit}
-    (heq : fourInputPosPos lhs l0 l1 r0 r1 = some (.and o0 o1)) :
-    o1.isConstant ∨ o1.var = lhs.var ∨ o1.var = l0.var ∨ o1.var = l1.var ∨ o1.var = r0.var ∨ o1.var = r1.var := by
-  grind [fourInputPosPos]
+theorem var_fourInputPosPos_and {lhs l0 l1 r0 r1 o0 o1 : Lit} (motive : Var -> Prop)
+    (heq : fourInputPosPos lhs l0 l1 r0 r1 = some (.and o0 o1))
+    (hlhs : motive lhs.var) (hr0 : motive r0.var) (hr1 : motive r1.var) :
+    motive o0.var ∧ motive o1.var := by
+  revert heq
+  generalize h : fourInputPosPos lhs l0 l1 r0 r1 = res
+  apply Option.of_wp_eq h
+  unfold fourInputPosPos
+  mvcgen with (cbv; grind)
 
 @[inline]
 def fourInputPosNeg (lhs l0 l1 r0 r1 : Lit) : Option SimplifiedAnd := do
@@ -283,63 +336,77 @@ theorem denote_fourInputPosNeg {lhs l0 l1 r0 r1 : Lit} {out : SimplifiedAnd}
     (heq : fourInputPosNeg lhs l0 l1 r0 r1 = some out)
     (hl : assign lhs = (assign l0 && assign l1)) :
     out.denote assign = (assign lhs && !(assign r0 && assign r1)) := by
-  simp [fourInputPosNeg] at heq
-  grind
+  revert heq
+  generalize h : fourInputPosNeg lhs l0 l1 r0 r1 = res
+  apply Option.of_wp_eq h
+  unfold fourInputPosNeg
+  mvcgen with (cbv; grind)
 
-@[grind →]
-theorem values_fourInputPosNeg_lit {lhs l0 l1 r0 r1 out : Lit}
-    (heq : fourInputPosNeg lhs l0 l1 r0 r1 = some (.lit out)) :
-    out.isConstant ∨ out.var = lhs.var ∨ out.var = l0.var ∨ out.var = l1.var ∨ out.var = r0.var ∨ out.var = r1.var := by
-  grind [fourInputPosNeg]
+theorem var_fourInputPosNeg_lit {lhs l0 l1 r0 r1 out : Lit} (motive : Var -> Prop)
+    (heq : fourInputPosNeg lhs l0 l1 r0 r1 = some (.lit out))
+    (hlhs : motive lhs.var) :
+    motive out.var := by
+  revert heq
+  generalize h : fourInputPosNeg lhs l0 l1 r0 r1 = res
+  apply Option.of_wp_eq h
+  unfold fourInputPosNeg
+  mvcgen with (cbv; grind)
 
-@[grind →]
-theorem values_fourInputPosNeg_and_lhs {lhs l0 l1 r0 r1 o0 o1 : Lit}
-    (heq : fourInputPosNeg lhs l0 l1 r0 r1 = some (.and o0 o1)) :
-    o0.isConstant ∨ o0.var = lhs.var ∨ o0.var = l0.var ∨ o0.var = l1.var ∨ o0.var = r0.var ∨ o0.var = r1.var := by
-  grind [fourInputPosNeg]
-
-@[grind →]
-theorem values_fourInputPosNeg_and_rhs {lhs l0 l1 r0 r1 o0 o1 : Lit}
-    (heq : fourInputPosNeg lhs l0 l1 r0 r1 = some (.and o0 o1)) :
-    o1.isConstant ∨ o1.var = lhs.var ∨ o1.var = l0.var ∨ o1.var = l1.var ∨ o1.var = r0.var ∨ o1.var = r1.var := by
-  grind [fourInputPosNeg]
+theorem var_fourInputPosNeg_and {lhs l0 l1 r0 r1 o0 o1 : Lit} (motive : Var -> Prop)
+    (heq : fourInputPosNeg lhs l0 l1 r0 r1 = some (.and o0 o1))
+    (hlhs : motive lhs.var) (hr0 : motive r0.var) (hr1 : motive r1.var) :
+    motive o0.var ∧ motive o1.var := by
+  revert heq
+  generalize h : fourInputPosNeg lhs l0 l1 r0 r1 = res
+  apply Option.of_wp_eq h
+  unfold fourInputPosNeg
+  mvcgen with (cbv; grind)
 
 @[inline]
-def fourInputNegNeg (l0 l1 r0 r1 : Lit) : Option SimplifiedAnd := do
+def fourInputNegNeg (l0 l1 r0 r1 : Lit) : Option Lit := do
   -- Resolution: ¬(l0 ∧ l1) ∧ ¬(l0 ∧ ¬l1) = ¬l0
-  if (l0 = r0 ∧ l1 = r1.invert) ∨ (l0 = r1 ∧ l1 = r0.invert) then
-    return .lit l0.invert
+  if (l0 = r0 ∧ l1 = r1.invert) then
+    return l0.invert
+
+  -- Resolution: ¬(l0 ∧ l1) ∧ ¬(¬l1 ∧ l0) = ¬l0
+  if (l0 = r1 ∧ l1 = r0.invert) then
+    return l0.invert
+
+  -- Resolution: ¬(l0 ∧ l1) ∧ ¬(l1 ∧ ¬l0) = ¬l1
+  if (l1 = r0 ∧ l0 = r1.invert) then
+    return l1.invert
 
   -- Resolution: ¬(l0 ∧ l1) ∧ ¬(¬l0 ∧ l1) = ¬l1
-  if (l1 = r0 ∧ l0 = r1.invert) ∨ (l1 = r1 ∧ l0 = r0.invert) then
-    return .lit l1.invert
+  if (l1 = r1 ∧ l0 = r0.invert) then
+    return l1.invert
 
   none
 
 include assignInv in
-theorem denote_fourInputNegNeg {l0 l1 r0 r1 : Lit} {out : SimplifiedAnd}
+theorem denote_fourInputNegNeg {l0 l1 r0 r1 : Lit} {out : Lit}
     (heq : fourInputNegNeg l0 l1 r0 r1 = some out) :
-    out.denote assign = (!(assign l0 && assign l1) && !(assign r0 && assign r1)) := by
-  simp [fourInputNegNeg] at heq
-  grind
+    assign out = (!(assign l0 && assign l1) && !(assign r0 && assign r1)) := by
+  revert heq
+  generalize h : fourInputNegNeg l0 l1 r0 r1 = res
+  apply Option.of_wp_eq h
+  unfold fourInputNegNeg
+  mvcgen
+  next h => simp only [Option.some.injEq]; intro h; cbv; grind only
+  next h => simp only [Option.some.injEq]; intro h; cbv; grind only
+  next h => simp only [Option.some.injEq]; intro h; cbv; grind only
+  next h => simp only [Option.some.injEq]; intro h; cbv; grind only
+  · cbv; grind
 
-@[grind →]
-theorem values_fourInputNegNeg_lit {l0 l1 r0 r1 out : Lit}
-    (heq : fourInputNegNeg l0 l1 r0 r1 = some (.lit out)) :
-    out.isConstant ∨ out.var = l0.var ∨ out.var = l1.var ∨ out.var = r0.var ∨ out.var = r1.var := by
-  grind [fourInputNegNeg]
 
-@[grind →]
-theorem values_fourInputNegNeg_and_lhs {l0 l1 r0 r1 o0 o1 : Lit}
-    (heq : fourInputNegNeg l0 l1 r0 r1 = some (.and o0 o1)) :
-    o0.isConstant ∨ o0.var = l0.var ∨ o0.var = l1.var ∨ o0.var = r0.var ∨ o0.var = r1.var := by
-  grind [fourInputNegNeg]
-
-@[grind →]
-theorem values_fourInputNegNeg_and_rhs {l0 l1 r0 r1 o0 o1 : Lit}
-    (heq : fourInputNegNeg l0 l1 r0 r1 = some (.and o0 o1)) :
-    o1.isConstant ∨ o1.var = l0.var ∨ o1.var = l1.var ∨ o1.var = r0.var ∨ o1.var = r1.var := by
-  grind [fourInputNegNeg]
+theorem var_fourInputNegNeg {l0 l1 r0 r1 out : Lit} (motive : Var -> Prop)
+    (heq : fourInputNegNeg l0 l1 r0 r1 = some out)
+    (hl0 : motive l0.var) (hl1 : motive l1.var) :
+    motive out.var := by
+  revert heq
+  generalize h : fourInputNegNeg l0 l1 r0 r1 = res
+  apply Option.of_wp_eq h
+  unfold fourInputNegNeg
+  mvcgen with (cbv; grind)
 
 @[inline]
 def fourInput (lhs rhs l0 l1 r0 r1 : Lit) : Option SimplifiedAnd :=
@@ -347,42 +414,54 @@ def fourInput (lhs rhs l0 l1 r0 r1 : Lit) : Option SimplifiedAnd :=
   | false, false => fourInputPosPos lhs l0 l1 r0 r1
   | false,  true => fourInputPosNeg lhs l0 l1 r0 r1
   | true,  false => fourInputPosNeg rhs r0 r1 l0 l1
-  | true,   true => fourInputNegNeg l0 l1 r0 r1
+  | true,   true => fourInputNegNeg l0 l1 r0 r1 |>.map .lit
 
-include assignInv assignFalse in
+include assignInv assignConst in
 theorem denote_fourInput {lhs rhs l0 l1 r0 r1 : Lit} {out : SimplifiedAnd}
     (heq : fourInput lhs rhs l0 l1 r0 r1 = some out)
-    (hl : assign lhs.strip = (assign l0 && assign l1))
-    (hr : assign rhs.strip = (assign r0 && assign r1)) :
+    (hl : assign lhs = ((decide lhs.inverted) ^^ (assign l0 && assign l1)))
+    (hr : assign rhs = ((decide rhs.inverted) ^^ (assign r0 && assign r1))) :
     out.denote assign = (assign lhs && assign rhs) := by
-  simp [fourInput] at heq
+  simp only [fourInput] at heq
   split at heq
-  · have := @denote_fourInputPosPos assign
-    grind
-  · have := @denote_fourInputPosNeg assign
-    grind
-  · have := @denote_fourInputPosNeg assign
-    grind
-  · have := @denote_fourInputNegNeg assign
-    grind
+  · rw [denote_fourInputPosPos assign heq (by simp_all)] <;> grind
+  · rw [denote_fourInputPosNeg assign heq (by simp_all)] <;> grind
+  · rw [denote_fourInputPosNeg assign heq (by simp_all)] <;> grind
+  · simp only [Option.map_eq_some_iff] at heq
+    rcases heq with ⟨res, ⟨heq, hlit⟩⟩
+    simp only [SimplifiedAnd.denote]
+    split
+    · simp only [SimplifiedAnd.lit.injEq] at hlit
+      rw [←hlit, denote_fourInputNegNeg assign heq]
+      <;> grind
+    · grind
 
-@[grind →]
-theorem values_fourInput_lit {lhs rhs l0 l1 r0 r1 out : Lit}
-    (heq : fourInput lhs rhs l0 l1 r0 r1 = some (.lit out)) :
-    out.isConstant ∨ out.var = lhs.var ∨ out.var = rhs.var ∨ out.var = l0.var ∨ out.var = l1.var ∨ out.var = r0.var ∨ out.var = r1.var := by
-  grind [fourInput]
+theorem var_fourInput_lit {lhs rhs l0 l1 r0 r1 out : Lit} (motive : Var -> Prop)
+    (heq : fourInput lhs rhs l0 l1 r0 r1 = some (.lit out))
+    (hconst : motive .constant)
+    (hlhs : motive lhs.var) (hrhs : motive rhs.var)
+    (hl0 : motive l0.var) (hl1 : motive l1.var) :
+    motive out.var := by
+  simp only [fourInput] at heq
+  split at heq
+  · grind [var_fourInputPosPos_lit motive]
+  · grind [var_fourInputPosNeg_lit motive]
+  · grind [var_fourInputPosNeg_lit motive]
+  · grind [var_fourInputNegNeg motive, Option.map_eq_some_iff]
 
-@[grind →]
-theorem values_fourInput_and_lhs {lhs rhs l0 l1 r0 r1 o0 o1 : Lit}
-    (heq : fourInput lhs rhs l0 l1 r0 r1 = some (.and o0 o1)) :
-    o0.isConstant ∨ o0.var = lhs.var ∨ o0.var = rhs.var ∨ o0.var = l0.var ∨ o0.var = l1.var ∨ o0.var = r0.var ∨ o0.var = r1.var := by
-  grind [fourInput]
 
-@[grind →]
-theorem values_fourInput_and_rhs {lhs rhs l0 l1 r0 r1 o0 o1 : Lit}
-    (heq : fourInput lhs rhs l0 l1 r0 r1 = some (.and o0 o1)) :
-    o1.isConstant ∨ o1.var = lhs.var ∨ o1.var = rhs.var ∨ o1.var = l0.var ∨ o1.var = l1.var ∨ o1.var = r0.var ∨ o1.var = r1.var := by
-  grind [fourInput]
+theorem var_fourInput_and {lhs rhs l0 l1 r0 r1 o0 o1 : Lit} (motive : Var -> Prop)
+    (heq : fourInput lhs rhs l0 l1 r0 r1 = some (.and o0 o1))
+    (hlhs : motive lhs.var) (hrhs : motive rhs.var)
+    (hl0 : motive l0.var) (hl1 : motive l1.var)
+    (hr0 : motive r0.var) (hr1 : motive r1.var) :
+    motive o0.var ∧ motive o1.var := by
+  simp only [fourInput] at heq
+  split at heq
+  · grind [var_fourInputPosPos_and motive]
+  · grind [var_fourInputPosNeg_and motive]
+  · grind [var_fourInputPosNeg_and motive]
+  · grind [Option.map_eq_some_iff]
 
 @[inline]
 def simplifyAnd (lhs rhs : Lit) (lin rin : Option (Lit × Lit)) : SimplifiedAnd := Id.run do
@@ -404,24 +483,67 @@ def simplifyAnd (lhs rhs : Lit) (lin rin : Option (Lit × Lit)) : SimplifiedAnd 
 
   return .and lhs rhs
 
-include assignInv assignFalse in
-theorem denote_simplifyAnd {lhs rhs : Lit} (lin rin : Option (Lit × Lit)) {out : SimplifiedAnd}
+include assignInv assignConst in
+theorem denote_simplifyAnd {lhs rhs : Lit} {lin rin : Option (Lit × Lit)} {out : SimplifiedAnd}
     (heq : simplifyAnd lhs rhs lin rin = some out)
-    (hl : ∀ {l0 l1}, lin = some (l0, l1) → assign lhs.strip = (assign l0 && assign l1))
-    (hr : ∀ {r0 r1}, rin = some (r0, r1) → assign rhs.strip = (assign r0 && assign r1)) :
+    (hl : ∀ {l0 l1}, lin = some (l0, l1) → assign lhs = (lhs.inverted ^^ (assign l0 && assign l1)))
+    (hr : ∀ {r0 r1}, rin = some (r0, r1) → assign rhs = (rhs.inverted ^^ (assign r0 && assign r1))) :
     out.denote assign = (assign lhs && assign rhs) := by
-  simp only [simplifyAnd] at heq
-  repeat' (split at heq; simp at heq)
-  · have := @denote_twoInput assign; grind only [= Id.run_pure, SimplifiedAnd.denote]
-  · have := @denote_threeInputLeft assign; grind only [= Id.run_pure, SimplifiedAnd.denote]
-  · have := @denote_threeInputLeft assign; grind only [= Id.run_pure, SimplifiedAnd.denote]
-  · have := @denote_fourInput assign; grind only [= Id.run_pure, SimplifiedAnd.denote]
-  · grind only [= Id.run_pure, SimplifiedAnd.denote]
-  · grind only [= Id.run_pure, SimplifiedAnd.denote]
-  · have := @denote_threeInputLeft assign; grind only [= Id.run_pure, SimplifiedAnd.denote]
-  · grind only [= Id.run_pure, SimplifiedAnd.denote]
-  · grind only [= Id.run_pure, SimplifiedAnd.denote]
-  · grind only [= Id.run_pure, SimplifiedAnd.denote]
+  have : some (.and lhs rhs) = some out → out.denote assign = (assign lhs && assign rhs) := by grind
+  revert heq
+  generalize h : simplifyAnd lhs rhs lin rin = res
+  apply Id.of_wp_run_eq h
+  mvcgen
+  <;> (intro h; simp only [Option.some.injEq] at h; rw [←h])
+  next heq => apply denote_twoInput assign heq <;> grind
+  next heq => apply denote_threeInputLeft assign heq <;> grind
+  next heq => rw [Bool.and_comm]; apply denote_threeInputLeft assign heq <;> grind
+  next heq => apply denote_fourInput assign heq <;> grind
+  next heq => apply denote_fourInput assign heq <;> grind
+  next heq => rw [Bool.and_comm]; apply denote_threeInputLeft assign heq <;> grind
+  next heq => apply denote_fourInput assign heq <;> grind
+  next => grind
+
+theorem var_simplifyAnd_lit {lhs rhs : Lit} {lin rin : Option (Lit × Lit)} {out : Lit} (motive : Var -> Prop)
+    (heq : simplifyAnd lhs rhs lin rin = some (SimplifiedAnd.lit out))
+    (hconst : motive .constant) (hlhs : motive lhs.var) (hrhs : motive rhs.var)
+    (hl : ∀ {l0 l1}, lin = some (l0, l1) → motive l0.var ∧ motive l1.var) :
+    motive out.var := by
+  revert heq
+  generalize h : simplifyAnd lhs rhs lin rin = res
+  apply Id.of_wp_run_eq h
+  have {lhs rhs} : some (SimplifiedAnd.and lhs rhs) = some (.lit out) → motive out.var := by grind only
+  mvcgen
+  <;> (try apply this)
+  <;> (intro h; simp [Option.some.injEq, SimplifiedAnd.lit.injEq] at h)
+  next heq => rw [←h]; apply var_twoInput motive heq <;> grind
+  next heq => rw [h] at heq; apply var_threeInputLeft_lit motive heq <;> grind
+  next heq => rw [h] at heq; apply var_threeInputLeft_lit motive heq <;> grind
+  next heq => rw [h] at heq; apply var_fourInput_lit motive heq <;> grind
+  next heq => rw [h] at heq; apply var_fourInput_lit motive heq <;> grind
+  next heq => rw [h] at heq; apply var_threeInputLeft_lit motive heq <;> grind
+  next heq => rw [h] at heq; apply var_fourInput_lit motive heq <;> grind
+  next => grind
+
+theorem var_simplifyAnd_and {lhs rhs o0 o1 : Lit} {lin rin : Option (Lit × Lit)} (motive : Var -> Prop)
+    (heq : simplifyAnd lhs rhs lin rin = some (SimplifiedAnd.and o0 o1))
+    (hlhs : motive lhs.var) (hrhs : motive rhs.var)
+    (hl : ∀ {l0 l1}, lin = some (l0, l1) → motive l0.var ∧ motive l1.var)
+    (hr : ∀ {r0 r1}, rin = some (r0, r1) → motive r0.var ∧ motive r1.var) :
+    motive o0.var ∧ motive o1.var := by
+  revert heq
+  generalize h : simplifyAnd lhs rhs lin rin = res
+  apply Id.of_wp_run_eq h
+  have : some (SimplifiedAnd.and lhs rhs) = some (.and o0 o1) → motive o0.var ∧ motive o1.var := by grind only
+  mvcgen
+  <;> (intro h; simp [Option.some.injEq] at h)
+  next heq => rw [h] at heq; apply var_threeInputLeft_and motive heq <;> grind
+  next heq => rw [h] at heq; apply var_threeInputLeft_and motive heq <;> grind
+  next heq => rw [h] at heq; apply var_fourInput_and motive heq <;> grind
+  next heq => rw [h] at heq; apply var_fourInput_and motive heq <;> grind
+  next heq => rw [h] at heq; apply var_threeInputLeft_and motive heq <;> grind
+  next heq => rw [h] at heq; apply var_fourInput_and motive heq <;> grind
+  next => grind
 
 end TwoLevelSimp
 end Valaig.Aig
